feat: sem eq def

CollapsingTowers/TwoLevelBasic/Erasure.lean
@@ -17,16 +17,16 @@ def erase : Expr → Expr
   | .let𝕔 b e => .lets (erase b) (erase e)
 
 @[simp]
-def eraseTy : Ty → Ty
+def erase_ty : Ty → Ty
   | .nat => .nat
-  | .arrow τa τb _ => .arrow (eraseTy τa) (eraseTy τb) ∅
-  | .fragment τ => eraseTy τ
-  | .rep τ => eraseTy τ
+  | .arrow τa τb _ => .arrow (erase_ty τa) (erase_ty τb) ∅
+  | .fragment τ => erase_ty τ
+  | .rep τ => erase_ty τ
 
 @[simp]
-def eraseTEnv : TEnv → TEnv
+def erase_env : TEnv → TEnv
   | [] => []
-  | (τ, _) :: Γ => (eraseTy τ, .stat) :: eraseTEnv Γ
+  | (τ, _) :: Γ => (erase_ty τ, .stat) :: erase_env Γ
 
 theorem erase_closed_at : ∀ e x, closed_at e x → closed_at (erase e) x :=
   by
@@ -74,7 +74,7 @@ theorem erase_open₀_comm : ∀ x e, erase (open₀ x e) = open₀ x (erase e) 
   by
   intros x e; apply erase_opening_comm
 
-theorem eraseTy_well_binding_time : ∀ 𝕊 τ, well_binding_time 𝕊 (eraseTy τ) :=
+theorem erase_ty_well_binding_time : ∀ 𝕊 τ, well_binding_time 𝕊 (erase_ty τ) :=
   by
   intros 𝕊 τ
   induction τ
@@ -89,14 +89,14 @@ theorem eraseTy_well_binding_time : ∀ 𝕊 τ, well_binding_time 𝕊 (eraseTy
   case fragment IH => apply IH
   case rep IH => apply IH
 
-theorem length_eraseTEnv : ∀ Γ, Γ.length = (eraseTEnv Γ).length :=
+theorem length_erase_env : ∀ Γ, Γ.length = (erase_env Γ).length :=
   by
   intros Γ
   induction Γ
   case nil => rfl
   case cons IH => simp; apply IH
 
-theorem binds_eraseTEnv : ∀ x τ 𝕊 Γ, binds x (τ, 𝕊) Γ → binds x ((eraseTy τ), .stat) (eraseTEnv Γ) :=
+theorem binds_erase_env : ∀ x τ 𝕊 Γ, binds x (τ, 𝕊) Γ → binds x ((erase_ty τ), .stat) (erase_env Γ) :=
   by
   intros x τ 𝕊 Γ Hbinds
   induction Γ
@@ -104,30 +104,30 @@ theorem binds_eraseTEnv : ∀ x τ 𝕊 Γ, binds x (τ, 𝕊) Γ → binds x ((
   case cons tails IH =>
     by_cases HEq : tails.length = x
     . simp [if_pos HEq] at Hbinds
-      simp [← length_eraseTEnv, if_pos HEq, Hbinds]
+      simp [← length_erase_env, if_pos HEq, Hbinds]
     . simp [if_neg HEq] at Hbinds
-      simp [← length_eraseTEnv, if_neg HEq]
+      simp [← length_erase_env, if_neg HEq]
       apply IH; apply Hbinds
 
-theorem erase_safety : ∀ Γ 𝕊 e τ φ, typing Γ 𝕊 e τ φ → typing (eraseTEnv Γ) .stat (erase e) (eraseTy τ) ∅ :=
+theorem erase_safety : ∀ Γ 𝕊 e τ φ, typing Γ 𝕊 e τ φ → typing (erase_env Γ) .stat (erase e) (erase_ty τ) ∅ :=
   by
   intros Γ 𝕊 e τ φ Hτ
   apply
     @typing.rec
-      (fun Γ 𝕊 e τ φ (H : typing Γ 𝕊 e τ φ) => typing (eraseTEnv Γ) .stat (erase e) (eraseTy τ) ∅)
-      (fun Γ e τ φ (H : typing_reification Γ e τ φ) => typing (eraseTEnv Γ) .stat (erase e) (eraseTy τ) ∅)
+      (fun Γ 𝕊 e τ φ (H : typing Γ 𝕊 e τ φ) => typing (erase_env Γ) .stat (erase e) (erase_ty τ) ∅)
+      (fun Γ e τ φ (H : typing_reification Γ e τ φ) => typing (erase_env Γ) .stat (erase e) (erase_ty τ) ∅)
   case fvar =>
     intros _ _ _ _ Hbinds _
     apply typing.fvar
-    apply binds_eraseTEnv; apply Hbinds
-    apply eraseTy_well_binding_time
+    apply binds_erase_env; apply Hbinds
+    apply erase_ty_well_binding_time
   case lam =>
     intros _ _ _ _ _ _ _ HwellBinds Hclose IH
     apply typing.lam
-    rw [← length_eraseTEnv, ← erase_open₀_comm]
+    rw [← length_erase_env, ← erase_open₀_comm]
     apply IH
-    apply eraseTy_well_binding_time
-    rw [← length_eraseTEnv]
+    apply erase_ty_well_binding_time
+    rw [← length_erase_env]
     apply erase_closed_at; apply Hclose
   case lift_lam =>
     intros _ _ _ _ _ _ _ IH
@@ -151,8 +151,8 @@ theorem erase_safety : ∀ Γ 𝕊 e τ φ, typing Γ 𝕊 e τ φ → typing (e
   case code_fragment =>
     intros _ x _ Hbinds HwellBinds
     apply typing.fvar
-    simp; apply binds_eraseTEnv; apply Hbinds
-    apply eraseTy_well_binding_time
+    simp; apply binds_erase_env; apply Hbinds
+    apply erase_ty_well_binding_time
   case code_rep =>
     intros _ _ _ _ IH
     apply IH
@@ -162,30 +162,30 @@ theorem erase_safety : ∀ Γ 𝕊 e τ φ, typing Γ 𝕊 e τ φ → typing (e
   case lam𝕔 =>
     intros _ _ _ _ _ _ _ Hclose IH
     apply typing.lam
-    rw [← length_eraseTEnv, ← erase_open₀_comm]
+    rw [← length_erase_env, ← erase_open₀_comm]
     apply IH
-    apply eraseTy_well_binding_time
-    rw [← length_eraseTEnv]
+    apply erase_ty_well_binding_time
+    rw [← length_erase_env]
     apply erase_closed_at; apply Hclose
   case lets =>
     intros _ _ _ _ _ _ _ _ _ _ _ Hclose IHb IHe
     rw [← union_pure_left ∅]
     apply typing.lets
     apply IHb
-    rw [← length_eraseTEnv, ← erase_open₀_comm]
+    rw [← length_erase_env, ← erase_open₀_comm]
     apply IHe
-    apply eraseTy_well_binding_time
-    rw [← length_eraseTEnv]
+    apply erase_ty_well_binding_time
+    rw [← length_erase_env]
     apply erase_closed_at; apply Hclose
   case let𝕔 =>
     intros _ _ _ _ _ _ _ _ HwellBinds Hclose IHb IHe
     rw [← union_pure_left ∅]
     apply typing.lets
     apply IHb
-    rw [← length_eraseTEnv, ← erase_open₀_comm]
+    rw [← length_erase_env, ← erase_open₀_comm]
     apply IHe
-    apply eraseTy_well_binding_time
-    rw [← length_eraseTEnv]
+    apply erase_ty_well_binding_time
+    rw [← length_erase_env]
     apply erase_closed_at; apply Hclose
   case run =>
     intros _ _ _ _ _ _ IH
@@ -198,7 +198,7 @@ theorem erase_safety : ∀ Γ 𝕊 e τ φ, typing Γ 𝕊 e τ φ → typing (e
     apply IH
   apply Hτ
 
-theorem erase_reification_safety : ∀ Γ e τ φ, typing_reification Γ e τ φ → typing_reification (eraseTEnv Γ) (erase e) (eraseTy τ) ∅ :=
+theorem erase_reification_safety : ∀ Γ e τ φ, typing_reification Γ e τ φ → typing_reification (erase_env Γ) (erase e) (erase_ty τ) ∅ :=
   by
   intros Γ e τ φ Hτ
   cases Hτ <;>
