CollapsingTowers/TwoLevelBasic/SemEquiv.lean
@@ -1,0 +1,119 @@
+
+import CollapsingTowers.TwoLevelBasic.Erasure
+abbrev Subst :=
+  List Expr
+
+@[simp]
+def multi_subst : Subst → Expr → Expr
+  | [], e => e
+  | v :: γ, e => subst (γ.length) v (multi_subst γ e)
+
+mutual
+@[simp]
+def sem_equiv_value : Expr → Expr → Ty → Prop
+  | .lit n₀, .lit n₁, .nat => n₀ = n₁
+  | .lam e₀, .lam e₁, (.arrow τ𝕒 τ𝕓 .pure) =>
+    ∀ v₀ v₁,
+      sem_equiv_value v₀ v₁ τ𝕒 →
+      sem_equiv_expr (open_subst v₀ e₀) (open_subst v₁ e₁) τ𝕓
+  | _, _, _ => false
+
+@[simp]
+def sem_equiv_expr (e₀ : Expr) (e₁ : Expr) (τ : Ty) : Prop :=
+    ∃ v₀ v₁,
+      stepn e₀ v₀ ∧
+      stepn e₁ v₁ ∧
+      sem_equiv_value v₀ v₁ τ
+end
+
+@[simp]
+def sem_equiv_env : Subst → Subst → TEnv → Prop
+  | [], [], [] => true
+  | v₀ :: γ₀, v₁ :: γ₁, (τ, .stat) :: Γ =>
+    sem_equiv_value v₀ v₁ τ ∧
+    sem_equiv_env γ₀ γ₁ Γ
+  | _, _, _ => false
+
+@[simp]
+def sem_equiv_typing (Γ : TEnv) (e₀ : Expr) (e₁ : Expr) (τ : Ty) : Prop :=
+  ∀ γ₀ γ₁,
+    sem_equiv_env γ₀ γ₁ Γ →
+    sem_equiv_expr (multi_subst γ₀ e₀) (multi_subst γ₁ e₁) τ
+
+theorem sem_equiv_value_lam :
+  ∀ f₀ f₁ τ𝕒 τ𝕓,
+    sem_equiv_value f₀ f₁ (.arrow τ𝕒 τ𝕓 .pure) →
+    ∃ e₀ e₁,
+      f₀ = .lam e₀ ∧ f₁ = .lam e₁ :=
+  by
+  intros f₀ f₁ τ𝕒 τ𝕓 H
+  cases f₀ <;> cases f₁ <;> simp at H
+  simp
+
+theorem fundamental :
+  ∀ Γ 𝕊 e τ φ,
+    typing Γ 𝕊 e τ φ →
+    sem_equiv_typing (erase_env Γ) (erase e) (erase e) (erase_ty τ) :=
+  by
+  intros Γ 𝕊 e τ φ Hτ
+  apply
+    @typing.rec
+      (fun Γ 𝕊 e τ φ (H : typing Γ 𝕊 e τ φ) =>
+          sem_equiv_typing (erase_env Γ) (erase e) (erase e) (erase_ty τ))
+      (fun Γ e τ φ (H : typing_reification Γ e τ φ) =>
+          sem_equiv_typing (erase_env Γ) (erase e) (erase e) (erase_ty τ))
+  case fvar =>
+    intros _ _ _ _ Hbinds _
+    admit
+  case lam =>
+    intros _ _ _ _ _ _ _ HwellBinds Hclose IH
+    admit
+  case lift_lam =>
+    intros _ _ _ _ _ _ _ IH
+    apply IH
+  case app₁ =>
+    intros _ _ _ _ _ _ _ _ _ _ _ IHf IHarg
+    intros γ₀ γ₁ semΓ
+    simp only [sem_equiv_typing, sem_equiv_expr] at IHarg IHf
+    have ⟨v₀, v₁, Hstepv₀, Hstepv₁, Hsem_value⟩ := IHarg γ₀ γ₁ semΓ
+    have ⟨f₀, f₁, Hstepf₀, Hstepf₁, Hsem_value_lam⟩ := IHf γ₀ γ₁ semΓ
+    have ⟨e₀, e₁, HEq₀, HEq₁⟩ := sem_equiv_value_lam f₀ f₁ _ _ Hsem_value_lam
+    rw [HEq₀, HEq₁, erase_ty, pure_empty, sem_equiv_value] at Hsem_value_lam
+    admit
+  case app₂ =>
+    intros _ _ _ _ _ _ _ _ _ IHf IHarg
+    admit
+  case lit =>
+    intros _ _ _
+    admit
+  case lift_lit =>
+    intros _ _ _ _ IH
+    apply IH
+  case code_fragment =>
+    intros _ x _ Hbinds HwellBinds
+    admit
+  case code_rep =>
+    intros _ _ _ _ IH
+    apply IH
+  case reflect =>
+    intros _ _ _ _ IH
+    apply IH
+  case lam𝕔 =>
+    intros _ _ _ _ _ _ _ Hclose IH
+    admit
+  case lets =>
+    intros _ _ _ _ _ _ _ _ _ _ _ Hclose IHb IHe
+    admit
+  case let𝕔 =>
+    intros _ _ _ _ _ _ _ _ HwellBinds Hclose IHb IHe
+    admit
+  case run =>
+    intros _ _ _ _ _ _ IH
+    apply IH
+  case pure =>
+    intros _ _ _ _ IH
+    apply IH
+  case reify =>
+    intros _ _ _ _ _ IH
+    apply IH
+  apply Hτ
